projection/proofs/to_cake/compilationProofScript.sml
@@ -1,7 +1,7 @@
 open preamble
 
 open  projectionTheory projectionProofTheory
-       chorSemTheory
+      chorSemTheory deadlockFreedomTheory
 
 open  payloadLangTheory payloadCongTheory payloadPropsTheory
       payload_to_cakemlProofTheory
@@ -92,7 +92,7 @@ Proof
   rw[net_find_is_some_lemma,projection_def,
      endpoint_to_choiceTheory.compile_network_def]
 QED
-        
+
 Theorem compilation_preservation:
   ∀s1 (c1 : chor) s2 c2    (* Chor *)
    conf p pSt1 pCd1 pEPN1  (* Payload *)
@@ -145,6 +145,70 @@ Proof
   >- rw [net_has_node_IS_SOME_net_find,IS_SOME_EXISTS]
   \\ asm_exists_tac
   \\ fs []
+QED
+
+
+Theorem compile_network_fv_net_end:
+  ∀l fv s. net_end (compile_network_fv fv (compile_network s chorLang$Nil l))
+Proof
+  Induct \\ EVAL_TAC
+  \\ rw [] \\ pop_assum (ASSUME_TAC o EVAL_RULE)
+  \\ rw []
+QED
+
+Theorem compile_network_conf_net_end:
+  ∀n conf. net_end n ⇒ net_end (compile_network conf n)
+Proof
+  Induct \\ EVAL_TAC \\ rw []
+  \\ pop_assum (ASSUME_TAC o EVAL_RULE)
+  \\ Cases_on ‘e’ \\ EVAL_TAC \\ rw []
+  \\ pop_assum (ASSUME_TAC o EVAL_RULE)
+  \\ rw []
+QED
+
+Theorem compilation_deadlock_freedom:
+  ∀s1 (c1 : chor)          (* Chor *)
+   conf p pSt1 pCd1 pEPN1  (* Payload *)
+   cSt1 vs1 env1.          (* CakeML *)
+   compile_network_ok s1 c1 (procsOf c1) ∧
+   conf.payload_size > 0   ∧
+   no_undefined_vars (s1,c1) ∧
+   no_self_comunication c1  ∧
+   (* new stuff *)
+   pEPN1 = projection conf s1 c1 (procsOf c1) ∧
+   net_find p pEPN1  = SOME (NEndpoint p pSt1 pCd1 ) ∧
+   cSt1.ffi.oracle = comms_ffi_oracle conf ∧
+   cSt1.ffi.ffi_state = (p,pSt1.queues,net_filter p pEPN1) ∧
+   (* payload_to_cakeml assumptions *)
+   pSt_pCd_corr pSt1 pCd1 ∧ (* Should be true by construction *)
+   sem_env_cor conf pSt1 env1 ∧
+   enc_ok conf env1 (letfuns pCd1) vs1
+   ⇒ ∃mc cSt2. (* CakeML *)
+      cEval_equiv conf
+        (evaluate (cSt1 with clock := mc) env1
+                        [compile_endpoint conf vs1 pCd1])
+        (cSt2 with clock := mc,Rval [Conv NONE []])
+Proof
+  rw []
+  \\ drule_all chor_deadlock_freedom
+  \\ rw []
+  \\ drule compilation_preservation_junkcong
+  \\ rpt (disch_then drule)
+  \\ rw []
+  \\ pop_assum drule_all
+  \\ rw []
+  \\ drule chor_to_endpointProofTheory.trans_s_nil
+  \\ rw []
+  \\ drule endpointPropsTheory.junkcong_net_end
+  \\ disch_then (mp_tac o fst o EQ_IMP_RULE)
+  \\ impl_tac >- fs[compile_network_fv_net_end]
+  \\ rw []
+  \\ drule_then (qspec_then ‘conf’ assume_tac) compile_network_conf_net_end
+  \\ drule_then (qspec_then ‘p’ mp_tac) net_end_net_find
+  \\ impl_tac >- fs [net_has_node_IS_SOME_net_find]
+  \\ rw []
+  \\ qpat_x_assum ‘cEval_equiv _ _ _’ (ASSUME_TAC o EVAL_RULE)
+  \\ asm_exists_tac \\ fs []
 QED
 
 val _ = export_theory ()
